proved a general version; although the mask is still a bit funky

sync.v
@@ -111,87 +111,77 @@ Section generic.
     Proof. apply _. Qed.
   
     Definition atomic_triple'
+               (α: val → iProp Σ)
                (β: val → A → A → val → iProp Σ)
                (Ei Eo: coPset)
                (f x: val) γ : iProp Σ :=
-      (∀ P Q, (∀ g g' r, (P ={Eo, Ei}=> gFrag γ g) ★
-                           (gFrag γ g' ★ β x g g' r ={Ei, Eo}=> Q r))
+      (∀ P Q, (∀ g, (P ={Eo, Ei}=> gFrag γ g ★ α x) ★
+                    (∀ g' r, gFrag γ g' ★ β x g g' r ={Ei, Eo}=> Q r))
               -★ {{ P }} f x {{ Q }})%I.
 
     Lemma update_a: ∀ x x': A, (gFullR x ⋅ gFragR x) ~~> (gFullR x' ⋅ gFragR x').
+    Proof. Admitted.
+
+    Definition sync : val :=
+      λ: "f_cons" "f_seq",
+        let: "l"  := "f_cons" #() in
+        let: "s" := mk_sync #() in
+        "s" ("f_seq" "l").
+
+    Definition seq_spec (f: val) (ϕ: val → A → iProp Σ) α β :=
+      ∀ (Φ: val → iProp Σ) (l: val),
+         {{ True }} f l {{ f', ■ (∀ (x: val) (Φ: val → iProp Σ) (g: A),
+                               heapN ⊥ N →
+                               heap_ctx ★ ϕ l g ★ α x ★ (∀ (v: val) (g': A), ϕ l g' -★ β x g g' v -★ |={⊤}=> Φ v)
+                               ⊢ WP f' x {{ Φ }} )}}.
+    
+    Definition cons_spec (f: val) (g: A) ϕ :=
+      ∀ Φ: val → iProp Σ,
+        (∀ (l: val) (γ: gname), ϕ l g -★ gFull γ g -★ gFrag γ g -★ Φ l)
+        ⊢ WP f #() {{ Φ }}.
+    
+    Lemma atomic_spec (f_cons f_seq: val) (ϕ: val → A → iProp Σ) α β:
+      ∀ (g0: A),
+        heapN ⊥ N → seq_spec f_seq ϕ α β → cons_spec f_cons g0 ϕ →
+        heap_ctx
+        ⊢ WP sync f_cons f_seq {{ f, ∃ γ, gFrag γ g0 ★ ∀ x, □ atomic_triple' α β ⊤ ⊤ f x γ  }}.
     Proof.
-      intros x x'.
-    Admitted.
-
-    Definition mk_sync' : val :=
-      λ: "init" "f_seq",
-        let: "l"  := "init" #() in
-        let: "lk" := newlock #() in
-          λ: "x",
-            acquire "lk";;
-            let: "v" := "f_seq" "l" "x" in
-            release "lk";;
-            "v".
-
-    Definition seq_spec (f: val) ϕ β :=
-      ∀ (x : val) (g g': A) (Φ: val → iProp Σ) (l: loc),
-        heapN ⊥ N →
-        heap_ctx ★ ϕ l g ★ (∀ r g', ϕ l g' -★ β x g g' r -★ Φ r)
-        ⊢ WP f #l x {{ Φ }}.
-    
-    Lemma atomic_spec (f_cons f_seq: val) ϕ β:
-      heapN ⊥ N → seq_spec f_seq ϕ β →
-      heap_ctx
-      ⊢ WP mk_sync' f_cons f_seq {{ f, ∃ γ, ∀ x, □ atomic_triple' β ⊤ ⊤ f x γ  }}.
-  Proof.
-    (* iIntros (HN) "#Hh". repeat wp_let. *)
-    (* wp_alloc l1 as "Hl1". *)
-    (* wp_alloc l2 as "Hl2". *)
-    (* iVs (own_alloc (gFullR (#0, #0) ⋅ gFragR (#0, #0))) as (γ) "Hγ"; first by done. *)
-    (* wp_let.  *)
-    (* iDestruct (own_op with "Hγ") as "[Hfull Hfrag]". *)
-    (* iAssert (∃ x1 x2, l1 ↦ x1 ★ l2 ↦ x2 ★ gFull γ (x1, x2))%I with "[-Hfrag]" as "HR". *)
-    (* { iExists #0, #0. by iFrame. } *)
-    (* wp_bind (newlock _). iApply newlock_spec=>//.  *)
-    (* iFrame "Hh".  *)
-    (* iFrame "HR". *)
-    (* iIntros (lk γ') "#Hlk". *)
-    (* wp_let.  *)
-    (* iClear "Hfrag". (* HFrag should be handled to user? *)  *)
-    (* iVsIntro. iExists γ. iAlways. *)
-    (* rewrite /is_pcas. *)
-    (* iIntros (a b P Q) "#H".  *)
-    (* iAlways. iIntros "HP". *)
-    (* repeat wp_let. *)
-    (* wp_bind (acquire _). *)
-    (* iApply acquire_spec. *)
-    (* iFrame "Hlk". iIntros "Hlked Hls". *)
-    (* iDestruct "Hls" as (x1 x2) "(Hl1 & Hl2 & HFulla)". *)
-    (* wp_seq. *)
-    (* wp_bind ((pcas_seq _) _). *)
-    (* iApply (pcas_seq_spec with "[Hlked HP Hl1 Hl2 HFulla]"); try auto. *)
-    (* iFrame "Hh". rewrite /ϕ. iCombine "Hl1" "Hl2" as "Hl". *)
-    (* instantiate (H2:=(x1, x2)). iFrame. *)
-    (* iIntros (v xs') "[Hl1 Hl2] Hβ". *)
-    (* wp_let. wp_bind (release _). wp_let. *)
-    (* iDestruct ("H" $! (x1, x2) xs' v) as "[Hvs1 Hvs2]". *)
-    (* iVs ("Hvs1" with "HP") as "Hfraga". (* XXX: this Hfraga might be too strong *) *)
-    (* iCombine "HFulla" "Hfraga" as "Ha". *)
-    (* iVs (own_update with "Ha") as "Hb". *)
-    (* { instantiate (H3:=(gFullR xs' ⋅ gFragR xs')). *)
-    (*   apply update_a. eauto. } *)
-    
-    (* (* I should have full access to lk now ... shit *) *)
-    (* iAssert (∃ lkl: loc, #lkl = lk ★ lkl ↦ #true)%I as "Hlkl". *)
-    (* { admit. } *)
-    (* iDestruct "Hlkl" as (lkl) "[% Hlkl]". subst. *)
-    (* wp_store. (* now I just simply discard the things ... *) *)
-    (* iDestruct (own_op with "Hb") as "[HFullb HFragb]". *)
-    (* iVs ("Hvs2" with "[Hβ HFragb]"). *)
-    (* { rewrite /gFrag. by iFrame. } *)
-    (* by iVsIntro. *)
-  Admitted.
-
+      iIntros (g0 HN Hseq Hcons) "#Hh". repeat wp_let.
+      wp_bind (f_cons _). iApply Hcons.
+      iIntros (l γ) "Hϕ HFull HFrag".
+      wp_let. wp_bind (mk_sync _).
+      iApply mk_sync_spec_wp=>//.
+      iAssert (∃ g: A, ϕ l g ★ gFull γ g)%I with "[-HFrag]" as "HR".
+      { iExists g0. by iFrame. }
+      iFrame "Hh HR".
+      iIntros (s) "#Hsyncer".
+      wp_let. rewrite /is_syncer /seq_spec.
+      wp_bind (f_seq _). iApply wp_wand_r. iSplitR; first by iApply (Hseq with "[]")=>//.
+      iIntros (f) "%".
+      iApply wp_wand_r. iSplitR; first by iApply "Hsyncer".
+      iIntros (v) "#Hrefines".
+      iExists γ. iFrame. iIntros (x).
+      iAlways. rewrite /atomic_triple'.
+      iIntros (P Q) "#Hvss".
+      rewrite /refines.
+      iDestruct "Hrefines" as "#Hrefines".
+      iSpecialize ("Hrefines" $! (of_val x) x P Q).
+      iApply ("Hrefines" with "[]"); first by rewrite to_of_val.
+      iAlways. iIntros "[HR HP]". iDestruct "HR" as (g) "[Hϕ HgFull]".
+      (* we should view shift at this point *)
+      iDestruct ("Hvss" $! g) as "[Hvs1 Hvs2]".
+      iApply pvs_wp.
+      iVs ("Hvs1" with "HP") as "[HgFrag Hα]".
+      iVsIntro.
+      iApply H0=>//. (* H0 name is horrible *)
+      iFrame "Hh Hϕ Hα". iIntros (ret g') "Hϕ' Hβ".
+      iCombine "HgFull" "HgFrag" as "Hg".
+      iVs (own_update with "Hg") as "[HgFull HgFrag]".
+      { apply update_a. }
+      iSplitL "HgFull Hϕ'".
+      - iExists g'. by iFrame.
+      - by iVs ("Hvs2" $! g' ret with "[HgFrag Hβ]"); first by iFrame.
+    Qed.
   End triple.
 End generic.
 
@@ -207,46 +197,54 @@ Section atomic_pair.
          else #false.
 
   Local Opaque pcas_seq.
-  
-  Definition ϕ (l1 l2: loc) (xs: val * val) : iProp Σ := (l1 ↦ fst xs ★ l2 ↦ snd xs)%I.
 
-  Definition β (a b: val) (xs xs': val * val) (v: val) : iProp Σ :=
-    (■ ((v = #true  ∧ fst xs = a ∧ snd xs = a ∧ fst xs' = b ∧ snd xs' = b) ∨
-        (v = #false ∧ (fst xs ≠ a ∨ snd xs ≠ a) ∧ xs = xs')))%I.
+  Definition α (x: val) : iProp Σ := (∃ a b: val, x = (a, b)%V)%I.
+  
+  Definition ϕ (ls: val) (xs: val * val) : iProp Σ :=
+    (∃ l1 l2: loc, ls = (#l1, #l2)%V ★ l1 ↦ fst xs ★ l2 ↦ snd xs)%I.
+
+  Definition β (ab: val) (xs xs': val * val) (v: val) : iProp Σ :=
+    (■ ∃ a b: val,
+         ab = (a, b)%V ∧
+         ((v = #true  ∧ fst xs = a ∧ snd xs = a ∧ fst xs' = b ∧ snd xs' = b) ∨
+          (v = #false ∧ (fst xs ≠ a ∨ snd xs ≠ a) ∧ xs = xs')))%I.
 
   Local Opaque β.
   
-  Lemma pcas_seq_spec (a b: val) (xs xs': val * val) ls:
-    ∀ (Φ: val → iProp Σ) (l1 l2: loc),
-      heapN ⊥ N → to_val ls = Some (#l1, #l2)%V →
-      heap_ctx ★ ϕ l1 l2 xs ★ (∀ v xs', ϕ l1 l2 xs' -★ β a b xs xs' v -★ Φ v)
-      ⊢ WP pcas_seq ls (a, b) {{ Φ }}.
+  Lemma pcas_seq_spec: seq_spec N pcas_seq ϕ α β.
   Proof.
-    rewrite /ϕ.
-    iIntros (Φ l1 l2 HN Hls) "(#Hh & (Hl1 & Hl2) & HΦ)".
-    wp_value. iVsIntro. 
-    wp_seq. repeat wp_let.
-    subst. wp_proj. wp_load.
-    wp_proj. wp_op=>[?|Hx1na].
+    rewrite /seq_spec.
+    intros Φ l.
+    iIntros "!# _". wp_seq. iVsIntro. iPureIntro. clear Φ.
+    iIntros (x Φ g HN) "(#Hh & Hg & Hα & HΦ)".
+    rewrite /ϕ /α.
+    iDestruct "Hg" as (l1 l2) "(% & Hl1 & Hl2)".
+    iDestruct "Hα" as (a b) "%".
+    subst. destruct g as (x1, x2). simpl.
+    wp_let. wp_proj. wp_load. wp_proj.
+    wp_op=>[?|Hx1na].
     - subst.
       wp_if. wp_proj. wp_load. wp_proj.
       wp_op=>[?|Hx2na]. subst.
       + wp_if. wp_proj. wp_proj. wp_store. wp_proj. wp_proj. wp_store.
-        iDestruct ("HΦ" $! #true (b, b)) as "H".
-        iApply ("H" with "[Hl1 Hl2]"); first by iFrame.
+        iDestruct ("HΦ" $! #true (b, b)) as "HΦ".
+        iApply ("HΦ" with "[Hl1 Hl2]").
+        { iExists l1, l2. by iFrame. }
         rewrite /β.
-        iPureIntro. left. eauto.
+        iPureIntro. exists a, b. split; first done. left. eauto.
       + wp_if.
-        iDestruct ("HΦ" $! #false xs) as "H".
-        iApply ("H" with "[Hl1 Hl2]"); first by iFrame.
+        iDestruct ("HΦ" $! #false (a, x2)) as "H".
+        iApply ("H" with "[Hl1 Hl2]").
+        { iExists l1, l2. by iFrame. }
         rewrite /β.
-        iPureIntro. right. eauto.
+        iPureIntro. exists a, b. split; first done. right. eauto.
     - subst.
       wp_if.
-      iDestruct ("HΦ" $! #false xs) as "H".
-      iApply ("H" with "[Hl1 Hl2]"); first by iFrame.
+      iDestruct ("HΦ" $! #false (x1, x2)) as "H".
+      iApply ("H" with "[Hl1 Hl2]").
+      { iExists l1, l2. by iFrame. }
       rewrite /β.
-      iPureIntro. right. eauto.
+      iPureIntro. exists a, b. split; first done. right. eauto.
   Qed.
 
   Definition is_pcas γ (f: val): iProp Σ :=
